theory/Sound_Communication_B.thy
@@ -1162,18 +1162,16 @@ lemma staticTraceablePoolSoundDynamicEval:
 staticLiveChanPool V Ln Lx xC [[] \<mapsto> Stt e Map.empty []] \<Longrightarrow>
 staticFlowsAcceptPool V F [[] \<mapsto> Stt e Map.empty []] \<Longrightarrow>
 star_left op \<rightarrow> ([[] \<mapsto> Stt e Map.empty []], {}) (Em, Hm) \<Longrightarrow>
-\<forall>\<pi>' e' env' stack' isEnd . 
-  Em \<pi>' = Some (Stt e' env' stack') \<longrightarrow>
-  dynamicBuiltOnChanTm env' (Ch \<pi>C xC) e' \<longrightarrow> (* need to generalize this (builtOnChan) (maybe deduce static version); it doesn't help for induction *)
-  isEnd (tmId e') \<longrightarrow>
-  (\<exists>path. pathsCongruentModChan (Em, Hm) (Ch \<pi>C xC) \<pi>' path \<and> staticTraceable F Ln Lx (IdBind xC) isEnd path) \<Longrightarrow>
-dynamicEval (Em, Hm) (E', H') \<Longrightarrow>
+(Em, Hm) \<rightarrow> (E', H') \<Longrightarrow>
 E' \<pi>' = Some (Stt e' env' stack') \<Longrightarrow>
-dynamicBuiltOnChanTm env' (Ch \<pi>C xC) e' \<Longrightarrow>
-isEnd (tmId e') \<Longrightarrow> 
-\<exists>path. pathsCongruentModChan (E', H') (Ch \<pi>C xC) \<pi>' path \<and> staticTraceable F Ln Lx (IdBind xC) isEnd path
+dynamicBuiltOnChanPool E' (Ch \<pi>C xC) \<Longrightarrow>
+\<forall>\<pi>' e'. (\<exists>env' stack'. Em \<pi>' = Some (Stt e' env' stack')) \<longrightarrow>
+        dynamicBuiltOnChanPool Em (Ch \<pi>C xC) \<longrightarrow>
+        (\<forall>isEnd. isEnd (tmId e') \<longrightarrow>
+                 (\<exists>path. pathsCongruentModChan (Em, Hm) (Ch \<pi>C xC) \<pi>' path \<and> staticTraceable F Ln Lx (IdBind xC) isEnd path)) \<Longrightarrow>
+isEnd (tmId e') \<Longrightarrow> \<exists>path. pathsCongruentModChan (E', H') (Ch \<pi>C xC) \<pi>' path \<and> staticTraceable F Ln Lx (IdBind xC) isEnd path
 "
-apply (erule dynamicEval.cases)
+apply (erule dynamicEval.cases; clarify)
 sorry
 
 lemma staticTraceablePoolSound':
@@ -1185,7 +1183,7 @@ staticFlowsAcceptPool V F [[] \<mapsto> (Stt e empty [])] \<Longrightarrow>
 \<forall> E' H' \<pi>' e' env' stack' isEnd .
   EH = ([[] \<mapsto> (Stt e empty [])], {}) \<longrightarrow> EH' = (E', H') \<longrightarrow>
   E' \<pi>' = Some (Stt e' env' stack') \<longrightarrow>
-  dynamicBuiltOnChanTm env' (Ch \<pi>C xC) e' \<longrightarrow>
+  dynamicBuiltOnChanPool E' (Ch \<pi>C xC) \<longrightarrow>
   isEnd (tmId e') \<longrightarrow>
   (\<exists> path .
     pathsCongruentModChan (E', H') (Ch \<pi>C xC) \<pi>' path \<and>
@@ -1193,16 +1191,17 @@ staticFlowsAcceptPool V F [[] \<mapsto> (Stt e empty [])] \<Longrightarrow>
 "
 apply (erule star_left.induct; clarify)
   using dynamicBuiltOnChanComplexNonEmpty
-  apply (metis map_upd_Some_unfold option.discI state.inject)
+  apply (smt dynamicBuiltOnChanPool.simps map_upd_Some_unfold option.discI state.inject)
   apply auto
   apply (rename_tac Em Hm E' H' \<pi>' e' env' stack' isEnd)
-  apply (erule staticTraceablePoolSoundDynamicEval; auto)
+  apply (erule staticTraceablePoolSoundDynamicEval; auto?)
 done
+
 
 lemma staticTraceablePoolSound:
 "
   \<E>' \<pi>' = Some (Stt e' \<rho>' \<kappa>') \<Longrightarrow>
-  dynamicBuiltOnChanTm \<rho>' (Ch \<pi>C xC) e' \<Longrightarrow>
+  dynamicBuiltOnChanPool \<E>' (Ch \<pi>C xC) \<Longrightarrow>
   star dynamicEval ([[] \<mapsto> (Stt e empty [])], {}) (\<E>', H') \<Longrightarrow>
   (V, C) \<Turnstile>\<^sub>\<E> [[] \<mapsto> (Stt e empty [])] \<Longrightarrow>
   staticLiveChanPool V Ln Lx xC [[] \<mapsto> (Stt e empty [])] \<Longrightarrow>
@@ -1220,7 +1219,7 @@ done
 
 lemma staticTraceableSound: "
   \<E>' \<pi>' = Some (Stt e' \<rho>' \<kappa>') \<Longrightarrow>
-  dynamicBuiltOnChanTm \<rho>' (Ch \<pi>C xC) e' \<Longrightarrow>
+  dynamicBuiltOnChanPool \<E>' (Ch \<pi>C xC) \<Longrightarrow>
   star dynamicEval ([[] \<mapsto> (Stt e empty [])], {}) (\<E>', H') \<Longrightarrow> 
   (V, C) \<Turnstile>\<^sub>e e \<Longrightarrow>
   staticLiveChan V Ln Lx xC e \<Longrightarrow>
@@ -1262,7 +1261,7 @@ lemma staticTraceableSendSound: "
  apply (frule_tac x\<^sub>s\<^sub>c = xsc and \<pi>C = \<pi>C and \<rho>\<^sub>e = enve in staticSendSiteSound; auto?)
   apply (frule staticTraceableSound; auto?)
   using dynamicBuiltOnChan_dynamicBuiltOnChanAtom_dynamicBuiltOnChanComplex_dynamicBuiltOnChanTm.Bind sendEvtBuiltOnChan 
-  apply blast
+  apply (meson dynamicBuiltOnChanPool.simps)
 done
 
 (* END PATH SOUND *)
